More bus reasoning

opentheory/theories/all.ml
@@ -37,6 +37,7 @@ loads "opentheory/theories/probability/probability.ml";;
 (* Natural number to bit-list conversions.                                   *)
 (* ------------------------------------------------------------------------- *)
 
+(***
 loads "opentheory/theories/natural-bits/natural-bits.ml";;
 
 (* ------------------------------------------------------------------------- *)
@@ -202,3 +203,4 @@ loads "opentheory/theories/haskell-char/haskell-char.ml";;
 (* ------------------------------------------------------------------------- *)
 
 loads "opentheory/theories/haskell-prime/haskell-prime.ml";;
+***)
